SSA/Experimental/Bits/AutoStructs/ForLean.lean
@@ -154,6 +154,11 @@ theorem Std.HashSet.mem_union [BEq α] [Hashable α] [LawfulBEq α] {m₁ m₂ :
   sorry
 
 @[simp]
+theorem Std.HashSet.isEmpty_union_iff_isEmpty [BEq α] [Hashable α] [LawfulBEq α] {m₁ m₂ : HashSet α} :
+    (m₁.union m₂).isEmpty ↔ m₁.isEmpty ∧ m₂.isEmpty := by
+  simp only [isEmpty_iff_forall_not_mem, mem_union, not_or, forall_and]
+
+@[simp]
 theorem Std.HashMap.mem_keysArray [BEq α] [Hashable α] [LawfulBEq α] [LawfulHashable α] {m : HashMap α β} {k : α} :
     k ∈ m.keysArray ↔ k ∈ m := by
   sorry
